{
 "cells": [
  {
   "cell_type": "markdown",
   "id": "3da4aa16",
   "metadata": {},
   "source": [
    "### 1.1.6.5. P6.2 ‚Äî Transformation on Function Spaces"
   ]
  },
  {
   "cell_type": "markdown",
   "id": "e41b3c40",
   "metadata": {},
   "source": [
    "$$\n",
    "V = \\left\\{ \\alpha\\, e^{2x}\\cos(x) + \\beta\\, e^{2x}\\sin(x) \\;\\middle|\\; \\alpha, \\beta \\in \\mathbb{R} \\right\\}\n",
    "$$\n",
    "\n",
    "$$\n",
    "L : V \\to V, \\quad L(f) = f' + f\n",
    "$$\n",
    "\n",
    "$$\n",
    "M_L = \\begin{bmatrix} 3 & 1 \\\\ -1 & 3 \\end{bmatrix}\n",
    "$$"
   ]
  },
  {
   "cell_type": "markdown",
   "id": "ec0fe9e2",
   "metadata": {},
   "source": [
    "**Explanation:**\n",
    "\n",
    "The vector space $V$ is spanned by $\\{e^{2x}\\cos(x),\\; e^{2x}\\sin(x)\\}$. The linear operator $L(f) = f' + f$ maps $V$ into itself. To find $M_L$, probe with each basis function and express the result in the same basis.\n",
    "\n",
    "**Example:**\n",
    "\n",
    "Let $f_1 = e^{2x}\\cos(x)$ and $f_2 = e^{2x}\\sin(x)$.\n",
    "\n",
    "$$\n",
    "f_1' = 2e^{2x}\\cos(x) - e^{2x}\\sin(x)\n",
    "$$\n",
    "\n",
    "$$\n",
    "L(f_1) = f_1' + f_1 = 3e^{2x}\\cos(x) - e^{2x}\\sin(x) = 3f_1 - f_2\n",
    "$$\n",
    "\n",
    "$$\n",
    "f_2' = 2e^{2x}\\sin(x) + e^{2x}\\cos(x)\n",
    "$$\n",
    "\n",
    "$$\n",
    "L(f_2) = f_2' + f_2 = e^{2x}\\cos(x) + 3e^{2x}\\sin(x) = f_1 + 3f_2\n",
    "$$\n",
    "\n",
    "$$\n",
    "M_L = \\begin{bmatrix} 3 & 1 \\\\ -1 & 3 \\end{bmatrix}\n",
    "$$"
   ]
  },
  {
   "cell_type": "code",
   "execution_count": null,
   "id": "f55f1480",
   "metadata": {},
   "outputs": [],
   "source": [
    "import sympy as sp\n",
    "\n",
    "x_sym = sp.Symbol(\"x\")\n",
    "\n",
    "basis_f1 = sp.exp(2 * x_sym) * sp.cos(x_sym)\n",
    "basis_f2 = sp.exp(2 * x_sym) * sp.sin(x_sym)\n",
    "\n",
    "l_f1 = sp.diff(basis_f1, x_sym) + basis_f1\n",
    "l_f2 = sp.diff(basis_f2, x_sym) + basis_f2\n",
    "\n",
    "l_f1_simplified = sp.expand(l_f1)\n",
    "l_f2_simplified = sp.expand(l_f2)\n",
    "\n",
    "print(f\"L(f1) = {l_f1_simplified}\")\n",
    "print(f\"L(f2) = {l_f2_simplified}\")\n",
    "\n",
    "coefficients_f1 = [l_f1_simplified.coeff(basis_f1), l_f1_simplified.coeff(basis_f2)]\n",
    "coefficients_f2 = [l_f2_simplified.coeff(basis_f1), l_f2_simplified.coeff(basis_f2)]\n",
    "\n",
    "matrix_l = sp.Matrix([[coefficients_f1[0], coefficients_f2[0]],\n",
    "                       [coefficients_f1[1], coefficients_f2[1]]])\n",
    "\n",
    "print(f\"\\nM_L =\\n{matrix_l}\")"
   ]
  },
  {
   "cell_type": "markdown",
   "id": "dff7f582",
   "metadata": {},
   "source": [
    "**References:**\n",
    "\n",
    "[üìò Savov, I. (2016). *No Bullshit Guide to Linear Algebra*, Problem P6.2.](https://minireference.com/static/excerpts/noBSLA_v2_preview.pdf)\n",
    "\n",
    "---\n",
    "\n",
    "[‚¨ÖÔ∏è Previous: P6.1 Image Space R¬≤ ‚Üí R¬≥](./02_p6_1_image_space_r2_to_r3.ipynb) | [Next: P6.3 Derivative on Polynomials ‚û°Ô∏è](./04_p6_3_derivative_on_polynomials.ipynb)"
   ]
  }
 ],
 "metadata": {
  "language_info": {
   "name": "python"
  }
 },
 "nbformat": 4,
 "nbformat_minor": 5
}
